Fomega/Proof.lean
@@ -15,7 +15,7 @@ namespace Fomega
   -- | lam_eta2 :
   --   Conv (Term.eta mf A t1) (.lam mf A t2) ->
   --   Conv t1 (.lam mf A t2)
-  | app_congr : Conv f1 f2 -> Conv a1 a2 -> Conv (.app m f1 a1) (.app m f2 a2)
+  | app_congr : Conv f1 f2 -> Conv a1 a2 -> Conv (.app mf f1 a1) (.app mf f2 a2)
   | app_beta1 : Conv (b β[t]) z -> Conv (.app mf (.lam mf A b) t) z
   | app_beta2 : Conv z (b β[t]) -> Conv z (.app mf (.lam mf A b) t)
 
